MAX_SPACE_SIZE = 1 << 29 again

theories/CertiGC/model/constants.v
@@ -11,7 +11,7 @@ Definition MAX_UINT: Z
 
 Definition MAX_SPACE_SIZE: Z
  := Eval cbv [Archi.ptr64]
- in if Archi.ptr64 then Z.shiftl 1 40 else Z.shiftl 1 28.
+ in if Archi.ptr64 then Z.shiftl 1 40 else Z.shiftl 1 29.
 
 Definition SPACE_STRUCT_SIZE: Z
  := Eval cbv [Archi.ptr64]
@@ -83,7 +83,12 @@ Qed.
 Lemma MSS_max_wordsize_signed_range (n: Z) (Hn: 0 <= n < MAX_SPACE_SIZE):
     Ptrofs.min_signed <= WORD_SIZE * n <= Ptrofs.max_signed.
 Proof.
-  pose proof WORD_SIZE_pos as HH.
-  split ; try rep_lia.
-  transitivity (WORD_SIZE * MAX_SPACE_SIZE) ; try nia ; try intro F ; try inversion F.
+  destruct Hn as [Hn_lo Hn_hi].
+  split.
+  - unfold WORD_SIZE.
+    transitivity 0 ; now try lia.
+  - rewrite Z.le_lteq.
+    left.
+    rewrite Z.lt_le_pred in Hn_hi.
+    apply Z.le_lt_trans with (WORD_SIZE * Z.pred MAX_SPACE_SIZE) ; unfold WORD_SIZE ; now try lia.
 Qed.
